

# Database Systems HW 1 for Question 4

Ishneet Kaur

February 3 2026

## 1 Question 4

You are given the following set  $F$  of functional dependencies for a relation  $R(A, B, C, D, E, F)$ .

$$F = \{A \rightarrow D, C \rightarrow BD, BD \rightarrow E, E \rightarrow CDF\}$$

Is  $AC \rightarrow CEF$  implied by  $F$ ? In other words, is  $AC \rightarrow CEF \in F^+$ ? If yes, use the inference rules to show how you can obtain this functional dependency from the dependencies in  $F$ .

### Solution

Yes,  $AC \rightarrow CEF$  is implied by  $F$ . This can be shown by computing the closure of  $AC$  and by using Armstrong's inference rules.

#### Part 1: Compute $(AC)^+$

With  $A \rightarrow D$ , we can add  $D$ :

$$(AC)^+ = \{A, C, D\}$$

With  $C$  now being in the closure, we can use the functional dependency  $C \rightarrow BD$  to add  $B$ :

$$(AC)^+ = \{A, B, C, D\}$$

With both attributes  $B$  and  $D$  in the closure, we can use the functional dependency  $BD \rightarrow E$  to add  $E$ :

$$(AC)^+ = \{A, B, C, D, E\}$$

With this updated closure, we can now use the functional dependency  $E \rightarrow CDF$  to add  $F$ :

$$(AC)^+ = \{A, B, C, D, E, F\}$$

Since all attributes are included in  $(AC)^+$  including  $CEF$ , we conclude:

$$AC \rightarrow CEF \in F^+$$

## Part 2: Inference Rules

We will now examine if the inference rules confirm  $AC \rightarrow CEF$

We will start with a given functional dependency.

Given:  $A \rightarrow D$

Next, we can use augmentation to add C to both sides as we want the left side to represent AC.

Augmentation:  $AC \rightarrow CD$

We can now decompose this to consolidate to the variables we are looking for on the right side.

Splitting:  $AC \rightarrow C$

With C now on the right side alone, we can use another given functional dependency.

Given:  $C \rightarrow BD$

We can now apply transitivity.

Transitivity:  $AC \rightarrow C$  and  $C \rightarrow BD$  so  $AC \rightarrow BD$

This now gives us another given functional dependency on the right.

Given:  $BD \rightarrow E$

We can apply transitivity again.

Transitivity:  $AC \rightarrow BD$  and  $BD \rightarrow E$  so  $AC \rightarrow E$

Now with all of the implications we have seen for AC, we can combine them to the right side.

Combining:  $AC \rightarrow C$  and  $AC \rightarrow BD$  and  $AC \rightarrow E$  so  $AC \rightarrow BCDE$

To get the last attribute, F, we can use another given functional dependency. For this, we can split to get the E which is on the left side of the functional dependency that will give us F.

Splitting:  $AC \rightarrow E$

Given:  $E \rightarrow CDF$

Transitivity:  $AC \rightarrow E$  and  $E \rightarrow CDF$  so  $AC \rightarrow CDF$

We can now combine everything together and see everything that  $AC$  implies.

Combining:  $AC \rightarrow BCDE$  and  $AC \rightarrow CDF$  so  $AC \rightarrow BCDEF$

To confirm the final answer, we can use splitting to get the exact attributes we are trying to validate.

Splitting:  $AC \rightarrow CEF$

### **Conclusion**

Therefore,  $AC \rightarrow CEF$  is implied by the given set of functional dependencies so

$$AC \rightarrow CEF \in F^+$$